\documentclass[a4paper, 10pt, english]{revtex4-2} %Add reprint for two columns

\usepackage[utf8]{inputenc}
\usepackage[english]{babel}

\usepackage{physics,amssymb}  % mathematical symbols (physics imports amsmath)
\usepackage{graphicx}         % include graphics such as plots
\usepackage{xcolor}           % set colors
\usepackage{hyperref}         % automagic cross-referencing (this is GODLIKE)
\usepackage{tikz}             % draw figures manually
%\usepackage{listings}         % display code
\usepackage{subfigure}        % imports a lot of cool and useful figure commands
\usepackage{array}
\usepackage{microtype}
\usepackage[export]{adjustbox}

\tolerance=1
\emergencystretch=\maxdimen
\hyphenpenalty=10000
\hbadness=10000

% defines the color of hyperref objects
% Blending two colors:  blue!80!black  =  80% blue and 20% black
\hypersetup{ % this is just my personal choice, feel free to change things
    colorlinks,
    linkcolor={red!50!black},
    citecolor={blue!50!black},
    urlcolor={blue!80!black}}

\newcommand{\txt}[1]{\text{#1}}
\newcommand{\parder}[2]{\frac{\partial #1}{\partial #2}}
\newcommand{\dder}[2]{\frac{\partial^2 #1}{\partial #2^2}}

\begin{document}
\vspace*{1.5cm}
\title{\LARGE Computational physics: Project 1}
\author{Jon Aleksander Pr√∏itz}
\date{\today}
\noaffiliation
\maketitle

\section*{\large Section 1}
    The local energy is given by
    \begin{equation}
            E_L 
        =   \frac{1}{\Psi_T}H\Psi_T
    \end{equation}
    with
    \begin{equation}
            H
        =   \sum_i^N \left(\frac{-\hbar^2}{2m} \nabla_i^2 + V_\txt{ext}\right) + \sum_{i<j}^N V_\txt{int}
    \end{equation}
    \begin{equation}
            V_{ext}(\mathbf{r}) 
        =   \Bigg\{
        \begin{array}{ll}
            \frac{1}{2}m\omega_{ho}^2r^2 & (S)\\
        \strut
            \frac{1}{2}m[\omega_{ho}^2(x^2+y^2) + \omega_z^2z^2] & (E)
        \label{trap_eqn}
        \end{array}
    \end{equation}
    \begin{equation}
        V_{int}(|\mathbf{r}_i-\mathbf{r}_j|) =  \Bigg\{
        \begin{array}{ll}
            \infty & {|\mathbf{r}_i-\mathbf{r}_j|} \leq {a}\\
            0 & {|\mathbf{r}_i-\mathbf{r}_j|} > {a}
        \end{array}
    \end{equation}
    \begin{equation}
        \Psi_T(\mathbf{r})=\Psi_T(\mathbf{r}_1, \mathbf{r}_2, \dots \mathbf{r}_N,\alpha,\beta)
        =\left[
           \prod_i g(\alpha,\beta,\mathbf{r}_i)
        \right]
        \left[
           \prod_{j<k}f(a,|\mathbf{r}_j-\mathbf{r}_k|)
        \right],
        \label{eq:trialwf}
    \end{equation}
    with 
    \begin{equation}
            g(\alpha, \beta, \mathbf{r}_i)
        =   exp\left[-\alpha\left(x_i^2+y_i^2+\beta z_i^2\right)\right]
    \end{equation}
    \begin{equation}
            f(a,|\mathbf{r}_i-\mathbf{r}_j|)=\Bigg\{
        \begin{array}{ll}
            0 & {|\mathbf{r}_i-\mathbf{r}_j|} \leq {a}\\
            (1-\frac{a}{|\mathbf{r}_i-\mathbf{r}_j|}) & {|\mathbf{r}_i-\mathbf{r}_j|} > {a}.
        \end{array}
    \end{equation}
    for $a=0$, $\beta = 1$, note that in one dimension for one particle
    \begin{equation}
            \frac{1}{\Psi_T}\dder{\Psi_T}{x}
        =   -2\alpha\frac{1}{\Psi_T}\parder{\Psi_T}{x}\left(x\Psi_T\right)
        =   2\alpha{\left(2\alpha x^2 - 1\right)}
    \end{equation}
    Due to the symmetric properties of the trial wavefunction we note that with $\nabla^2 = \sum_{i=1}\dder{}{x_i}$
    \begin{equation}
            \frac{1}{\Psi_T} \sum_{i=1}^d \dder{\Psi_T}{x_i}
        =   2\alpha\left(2\alpha\sum_{i=1}^dx_i^2 - d\right)
        =   2\alpha\left(2\alpha r^2 - d\right)
    \end{equation}
    where $d$ is the number of dimensions. Hence
    \begin{equation}
            E_L
        =   \sum_i^N\left(\frac{-\hbar^2}{2m}2\alpha\left(2\alpha r_i^2 - d\right) + \frac{1}{2}m\omega_{ho}^2r_i^2\right)
        =   \sum_i^N\frac{d}{2}\hbar\omega_{ho}
        =   \frac{Nd}{2}\hbar\omega_{ho}
    \end{equation}
    with $\alpha = 1/2a_{ho}^2$ and $a_{ho} = \sqrt{\hbar/m\omega_{ho}}$
    \begin{equation}
            \mathbf{F}
        =   \frac{2\nabla \Psi_T}{\Psi_T}
        =   -4\alpha \sum_{i=1}^d x_i \hat{\mathbf{x}_i}
    \end{equation}

    Define $g(\alpha, \beta, \mathbf{r}_i) = \phi(\mathbf{r}_i)$ and $r_{jm} = |\mathbf{r}_j - \mathbf{r}_m|$, such that
    \begin{equation}
            \Psi_T 
        =   \left[\prod_i\phi(\mathbf{r}_i)\right] e^{\sum_{j<m} \ln{f(r_{jm})}}
        =   \left[\prod_i\phi(\mathbf{r}_i)\right] e^{\sum_{j<m} u(r_{jm})}
    \end{equation}
    with $u(r_{jm}) = \ln{f(r_{jm})}$. The derivative of particle $k$ is then
    \begin{equation}
            \nabla_k\Psi_T 
        =   \nabla_k\left[\prod_i \phi(\mathbf{r}_i)\right]e^{\sum_{j<m} u(_{jm})} + \left[\prod_i\phi(\mathbf{r}_i)\right] \nabla_k\left(e^{\sum_{j<m} u(r_{jm})}\right)
    \end{equation}
    we note that in the frist term only particle $k$ is affected by the derivation, such that
    \begin{equation}
            \nabla_k\prod_i \phi(\mathbf{r}_i) 
        =   \nabla_k\phi(\mathbf{r}_i)\left[\prod_{i\neq k}\phi(\mathbf{r}_i)\right]
    \end{equation}
    while the second term
    \begin{equation}
                \nabla_k\left(e^{\sum_{j<m} u(r_{jm})}\right)
            =   e^{\sum_{j<m} u(r_{jm})} \nabla_k\sum_{j<m}u(r_{jm})
            =   e^{\sum_{j<m} u(r_{jm})} \sum_{k\neq l}\nabla_k u(r_{kl})
    \end{equation}
    such that
    \begin{equation}
            \nabla_k\Psi_T 
        =   \nabla_k\phi(\mathbf{r}_i)\left[\prod_{i\neq k}\phi(\mathbf{r}_i)\right] e^{\sum_{j<m} u(r_{jm})} + \left[\prod_i\phi(\mathbf{r}_i)\right] e^{\sum_{j<m} u(r_{jm})} \sum_{k\neq l}\nabla_k u(r_{kl})
    \end{equation}     




\end{document}
